typeclass/typing/pure_tcexp_typingScript.sml
@@ -1,0 +1,311 @@
+open HolKernel Parse boolLib bossLib BasicProvers dep_rewrite;
+open pairTheory arithmeticTheory integerTheory stringTheory optionTheory
+     listTheory alistTheory relationTheory set_relationTheory pred_setTheory;
+open typeclass_typesTheory pure_tcexpTheory typeclass_texpTheory
+typeclass_kindCheckTheory pure_configTheory;
+open monadsyntax;
+open typeclass
+
+val _ = monadsyntax.enable_monadsyntax();
+val _ = monadsyntax.enable_monad "option";
+
+val _ = new_theory "pure_tcexp_typing";
+
+Type tcexp_typedef[pp] = ``:Kind list # ((mlstring # type_kind_scheme list) list)``;
+Type tcexp_typedefs[pp] = ``:tcexp_typedef list``;
+Type tcexp_namespace[pp] = ``:exndef # tcexp_typedefs``;
+
+Definition namespace_to_tcexp_namespace_def:
+  namespace_to_tcexp_namespace (ns:exndef # typedefs) =
+    ((FST ns,MAP (I ## MAP (I ## MAP ($, []))) (SND ns))):tcexp_namespace
+End
+
+Definition type_scheme_ok_def:
+  type_scheme_ok (typedefs: tcexp_typedefs) ks
+    ((varks,t):type_kind_scheme) =
+  kind_ok typedefs (varks ++ ks) kindType t
+End
+
+Definition tcexp_namespace_ok_def:
+  tcexp_namespace_ok (exndef : exndef, typedefs : tcexp_typedefs) ⇔
+    (* No empty type definitions: *)
+      EVERY (λ(ak,td). td ≠ []) typedefs ∧
+    (* Unique, unreserved constructor names: *)
+      ALL_DISTINCT
+        (MAP implode (SET_TO_LIST (reserved_cns DELETE "Subscript")) ++
+         MAP FST exndef ++ MAP FST (FLAT $ MAP SND typedefs)) ∧
+    (* Every constructor type is closed wrt kinds and uses only defined
+       types: *)
+      EVERY (λ(ak,td).
+        EVERY (λ(cn,argtys). EVERY (type_scheme_ok typedefs ak) argtys) td) typedefs ∧
+    (* Every exception constructor type is closed and uses only defined types: *)
+      EVERY (λ(cn,tys). EVERY (type_ok typedefs []) tys) exndef ∧
+    (* Subscript is a valid exception *)
+      MEM («Subscript»,[]) exndef
+End
+
+Definition tcexp_type_cons_def:
+  tcexp_type_cons (typedefs:tcexp_typedefs) db (cname,carg_tys:type_kind_scheme list) (tyid,tyargs) ⇔
+    ∃argks constructors schemes.
+      (* There is some type definition: *)
+        oEL tyid typedefs = SOME (argks, constructors) ∧
+      (* Which declares the constructor: *)
+        ALOOKUP constructors cname = SOME schemes ∧
+      (* And we can specialise it appropriately: *)
+        LIST_REL (kind_ok typedefs db) argks tyargs ∧
+        LIST_REL (λ(ks,scheme) (ks',carg_t).
+          ks = ks' ∧
+          subst_db (LENGTH ks) tyargs scheme = carg_t
+          ) schemes carg_tys
+End
+
+Definition tcexp_destruct_type_cons_def:
+  tcexp_destruct_type_cons (edef:exndef,tdefs: tcexp_typedefs) db t cname carg_tys ⇔
+  if t = Atom Exception
+  then
+    EVERY (\x. FST x = []) carg_tys ∧
+    type_exception edef (cname,MAP SND carg_tys)
+  else
+  ∃tc targs.
+    split_ty_head t = SOME (tc,targs) ∧
+    case tc of
+    | INL tyid => tcexp_type_cons tdefs db (cname,carg_tys) (tyid,targs)
+    | INR (PrimT Bool) => MEM cname [«True»;«False»] ∧ carg_tys = []
+    | INR (CompPrimT (Tuple n)) => cname = «» ∧ MAP ($, []) targs = carg_tys
+    | _ => F
+End
+
+Definition get_constructors_def:
+  get_constructors (edef:exndef,tdefs) t ⇔
+  if t = Atom Exception
+  then SOME $ MAP (I ## LENGTH) edef
+  else do
+    (tc,targs) <- split_ty_head t;
+    case tc of
+    | INL tyid => OPTION_MAP (MAP (I ## LENGTH) o SND) $ oEL tyid tdefs
+    | INR (PrimT Bool) => SOME ([«True»,0;«False»,0])
+    | INR (CompPrimT (Tuple n)) => SOME ([«»,n])
+    | _ => NONE
+  od
+End
+
+Inductive tcexp_type_cepat:
+[~Var:]
+  tcexp_type_cepat ns db (cepatVar v) (tk:type_kind_scheme) [(v,tk)]
+
+[~UScore:]
+  tcexp_type_cepat ns db cepatUScore (tk:type_kind_scheme) []
+
+[~Cons:]
+  tcexp_destruct_type_cons ns db t c ts ∧
+  LIST_REL3 (tcexp_type_cepat ns db) pats ts vtss ⇒
+    tcexp_type_cepat ns db (cepatCos c pats) ([],t) (FLAT vtss)
+End
+
+Inductive tcexp_exhaustive_cepat:
+[~Var:]
+  cepatVar v ∈ pats ⇒
+    tcexp_exhaustive_cepat ns db (tk:type_kind_scheme) pats
+
+[~UScore:]
+  cepatUScore ∈ pats ⇒
+    tcexp_exhaustive_cepat ns db tk pats
+
+[~Cons:]
+  (∀c ts. tcexp_destruct_type_cons ns db t c ts ⇒
+    ∃(pss:cepat list set).
+      tcexp_exhaustive_cepatl ns db ts pss ∧ IMAGE (cepat c) pss ⊆ pats) ⇒
+  tcexp_exhaustive_cepat ns db ([],t) pats
+
+[~Nil:]
+  [] ∈ pss ⇒
+    tcexp_exhaustive_cepatl ns db [] pss
+
+[~List:]
+  tcexp_exhaustive_cepat ns db tk hs ∧ 
+  tcexp_exhaustive_cepatl ns db ts tls ∧
+  IMAGE (UNCURRY CONS) (hs × tls) ⊆ pss ⇒
+    tcexp_exhaustive_cepatl ns db (tk::ts) pss
+End
+
+(* typing rules for tcexp (expressions after dictionary construction) *)
+Inductive type_tcexp:
+[~Var:]
+  (ALOOKUP env x = SOME s ∧ specialises (SND ns) db s t ⇒
+      type_tcexp (ns:tcexp_namespace) db st env (pure_tcexp$Var x) t)
+
+[~Tuple:]
+  (LIST_REL (type_tcexp ns db st env) es ts ⇒
+      type_tcexp ns db st env (Prim (Cons «») es)
+        (cons_types (Atom $ CompPrimTy $ Tuple $ LENGTH ts) ts))
+
+[~Ret:]
+  (type_tcexp ns db st env e t ⇒
+      type_tcexp ns db st env (Prim (Cons «Ret») [e]) (Monad t))
+
+[~Bind:]
+  (type_tcexp ns db st env e1 (Monad t1) ∧
+   type_tcexp ns db st env e2 (Functions [t1] (Monad t2)) ⇒
+      type_tcexp ns db st env (Prim (Cons «Bind») [e1;e2]) (Monad t2))
+
+[~Raise:]
+  (type_tcexp ns db st env e (Atom Exception) ∧
+   type_ok (SND ns) db t ⇒
+      type_tcexp ns db st env (Prim (Cons «Raise») [e]) (Monad t))
+
+[~Handle:]
+  (type_tcexp ns db st env e1 (Monad t) ∧
+   type_tcexp ns db st env e2 (Functions [Atom Exception] (Monad t)) ⇒
+      type_tcexp ns db st env (Prim (Cons «Handle») [e1;e2]) (Monad t))
+
+[~Act:]
+  (type_tcexp ns db st env e (Atom $ PrimTy Message) ⇒
+      type_tcexp ns db st env (Prim (Cons «Act») [e]) (Monad $ Atom $ PrimTy String))
+
+[~Alloc:]
+   type_tcexp ns db st env e1 (Atom $ PrimTy Integer) ∧
+   type_tcexp ns db st env e2 t ⇒
+      type_tcexp ns db st env (Prim (Cons «Alloc») [e1;e2])
+        (Monad $ Cons (Atom $ CompPrimTy $ Array) t)
+
+[~Length:]
+   type_tcexp ns db st env e (Cons (Atom $ CompPrimTy $ Array) t) ⇒
+      type_tcexp ns db st env (Prim (Cons «Length») [e]) (Monad $ Atom $ PrimTy Integer)
+
+[~Deref:]
+   type_tcexp ns db st env e1 (Cons (Atom $ CompPrimTy $ Array) t) ∧
+   type_tcexp ns db st env e2 (Atom $ PrimTy Integer) ⇒
+      type_tcexp ns db st env (Prim (Cons «Deref») [e1;e2]) (Monad t)
+
+[~Update:]
+   type_tcexp ns db st env e1 (Cons (Atom $ CompPrimTy $ Array) t) ∧
+   type_tcexp ns db st env e2 (Atom $ PrimTy Integer) ∧
+   type_tcexp ns db st env e3 t ⇒
+      type_tcexp ns db st env (Prim (Cons «Update») [e1;e2;e3]) (Monad Unit)
+
+[~Exception:]
+   LIST_REL (type_tcexp (exndef,typedefs) db st env) es earg_ts ∧
+   type_exception exndef (cname,earg_ts) ⇒
+      type_tcexp ns db st env (Prim (Cons cname) es) (Atom Exception)
+
+[~True:]
+   type_tcexp ns db st env (Prim (Cons «True») []) (Atom $ PrimTy Bool)
+
+[~False:]
+   type_tcexp ns db st env (Prim (Cons «False») []) (Atom $ PrimTy Bool)
+
+[~Cons:]
+   LIST_REL (λe (ks,t).
+      type_tcexp ns (ks ++ db)
+        (MAP (tshift (LENGTH ks)) st)
+        (tshift_env (LENGTH ks) env) e t)
+      es (carg_ts: type_kind_scheme list) ∧
+   EVERY (type_ok (SND ns) db) tyargs ∧
+   tcexp_type_cons (SND ns) db (cname,carg_ts) (tyid,tyargs) ⇒
+      type_tcexp ns db st env
+        (Prim (Cons cname) es) (tcons_to_type (INL tyid) tyargs)
+
+[~Loc:]
+   oEL n st = SOME t ⇒
+      type_tcexp ns db st env (Prim (AtomOp $ Lit (Loc n)) [])
+        (Cons (Atom $ CompPrimTy $ Array) t)
+
+[~AtomOp:]
+   LIST_REL (type_tcexp ns db st env) es ts ∧
+   get_PrimTys ts = SOME pts ∧
+   type_atom_op aop pts pt ⇒
+      type_tcexp ns db st env (Prim (AtomOp aop) es) (Atom $ PrimTy pt)
+
+[~Seq:]
+  (type_tcexp ns db st env e1 t1 ∧ type_tcexp ns db st env e2 t2 ⇒
+      type_tcexp ns db st env (Prim Seq [e1; e2]) t2)
+
+[~App:]
+  (type_tcexp ns db st env e (Functions arg_tys ret_ty) ∧
+   LIST_REL (type_tcexp ns db st env) es arg_tys ∧ arg_tys ≠ [] ⇒
+      type_tcexp ns db st env (App e es) ret_ty)
+
+[~Lam:]
+  (EVERY (type_ok (SND ns) db) arg_tys ∧
+   LENGTH arg_tys = LENGTH xs ∧ arg_tys ≠ [] ∧
+   type_tcexp ns db st (REVERSE (ZIP (xs, MAP ($, []) arg_tys)) ++ env) e ret_ty
+      ⇒ type_tcexp ns db st env (Lam xs e) (Functions arg_tys ret_ty))
+
+[~Let:]
+   LENGTH new = n ∧
+   type_tcexp ns (new ++ db) (MAP (tshift n) st) (tshift_env n env) e1 t1 ∧
+   type_tcexp ns db st ((x,new,t1)::env) e2 t2 ⇒
+      type_tcexp ns db st env (Let x e1 e2) t2
+
+[~Letrec:]
+   LIST_REL
+    (λ(fn,body) (vars,scheme).
+      type_tcexp ns (vars ++ db) (MAP (tshift $ LENGTH vars) st)
+        (tshift_env (LENGTH vars) $
+          REVERSE (ZIP (MAP FST fns,schemes)) ++ env)
+        body scheme)
+    fns schemes ∧
+   EVERY (type_kind_scheme_ok (SND ns) db) schemes ∧ fns ≠ [] ∧
+   type_tcexp ns db st (REVERSE (ZIP (MAP FST fns, schemes)) ++ env) e t ⇒
+      type_tcexp ns db st env (Letrec fns e) t
+
+[~NestedCase:]
+  type_tcexp ns db st env e vt ∧
+  EVERY (λ(p,e).
+    ∃vts. tcexp_type_cepat ns db p ([],vt) vts ∧
+    type_tcexp ns db st
+      (REVERSE vts ++ ((v,[],vt)::env))
+      e t) ((p,e1)::pes) ∧
+  tcexp_exhaustive_cepat ns db ([],vt) (p INSERT (IMAGE FST $ set pes)) ∧
+  ¬MEM v (FLAT (MAP (cepat_vars_l ∘ FST) ((p,e1)::pes))) ⇒
+    type_tcexp ns db st env (NestedCase e v p e1 pes) t
+
+[~Case:]
+   type_tcexp ns db st env e vt ∧
+
+   (* get the list of constructors and their arities *)
+   get_constructors ns vt = SOME constructors ∧
+
+   (* no catch-all case *)
+   (usopt = NONE ⇒
+      (* exhaustive pattern-match *)
+        set (MAP FST css) = set (MAP FST constructors) ∧
+      (* no duplicated patterns *)
+        ALL_DISTINCT (MAP FST css)) ∧
+
+   (* catch-all case *)
+   (∀us_cn_ars us_e. usopt = SOME (us_cn_ars, us_e) ⇒
+      (* exhaustive pattern-match *)
+        set (MAP FST css) ∪ set (MAP FST us_cn_ars) = set (MAP FST constructors) ∧
+      (* no duplicated patterns *)
+        ALL_DISTINCT (MAP FST css ++ MAP FST us_cn_ars) ∧
+      (* non-empty cases/underscore patterns *)
+        css ≠ [] ∧ us_cn_ars ≠ [] ∧
+      (* all underscore patterns are valid *)
+        EVERY (λ(cn,ar).
+          ALOOKUP constructors cn = SOME ar) us_cn_ars ∧
+      (* continuation is well-typed *)
+        type_tcexp ns db st ((v,[],vt)::env) us_e t) ∧
+
+   (* For each case: *)
+   EVERY (λ(cname,pvars,cexp).
+      ∃ptys.
+        tcexp_destruct_type_cons ns db vt cname ptys ∧
+        (* Pattern variables do not shadow case split and are distinct: *)
+          ¬ MEM v pvars ∧ ALL_DISTINCT pvars ∧
+        (* Continuation is well-typed: *)
+          type_tcexp ns db st
+            (REVERSE (ZIP (pvars, ptys)) ++
+             (v,[],vt)::env)
+            cexp t
+      ) css ⇒
+      type_tcexp ns db st env (Case e v css usopt) t
+
+[~SafeProj:]
+   type_tcexp ns (ks ++ db) (MAP (tshift $ LENGTH ks) st)
+    (tshift_env (LENGTH ks) env) e t' ∧
+   tcexp_destruct_type_cons ns db t cname tys ∧
+   LENGTH tys = arity ∧ i < arity ∧ EL i tys = (ks,t') ⇒
+     type_tcexp ns db st env (SafeProj cname arity i e) t
+End
+
