typeclass/typing/typeclass_texpScript.sml
@@ -11,7 +11,8 @@ val _ = new_theory "typeclass_texp";
 (* We associate a poly-type to variable.
 * This is needed for type elaboration.
 * It can be provided by the user as well. *)
-Type annot_cvname = ``:(cvname # (num # PredType) option)``;
+(* 'a can be instantiated to Kind list or num *)
+Type annot_cvname = ``:(cvname # ('a # PredType) option)``;
 Type class_constr = ``:(cvname # type)``;
 
 Datatype:
@@ -21,8 +22,8 @@ Datatype:
         | Prim cop (texp list)                        (* primitive operations     *)
         | App texp (texp list)                       (* function application     *)
         | Lam ((cvname # (type option)) list) texp    (* lambda                   *)
-        | Let annot_cvname texp texp                 (* let                      *)
-        | Letrec ((annot_cvname # texp) list) texp   (* mutually recursive exps  *)
+        | Let ('a annot_cvname) texp texp                 (* let                      *)
+        | Letrec (('a annot_cvname # texp) list) texp   (* mutually recursive exps  *)
         | UserAnnot type texp                         (* user type annotation     *)
         | NestedCase texp cvname cepat texp
             ((cepat # texp) list)                     (* case of                  *)
@@ -30,11 +31,11 @@ End
 
 (* top level declarations *)
 Datatype:
-  tcdecl = FuncDecl PredType texp (* enforce top level declarations *)
+  tcdecl = FuncDecl PredType ('a texp) (* enforce top level declarations *)
 End
 
 Definition freevars_texp_def[simp]:
-  freevars_texp ((Var c v): texp) = {v} /\
+  freevars_texp ((Var c v): 'a texp) = {v} /\
   freevars_texp (Prim op es) = BIGUNION (set (MAP (λa. freevars_texp a) es)) /\
   freevars_texp (App e es) =
     freevars_texp e ∪ BIGUNION (set (MAP freevars_texp es)) ∧
@@ -51,7 +52,7 @@ Definition freevars_texp_def[simp]:
     DELETE gv) ∧
   freevars_texp (UserAnnot t e) = freevars_texp e
 Termination
-  WF_REL_TAC `measure texp_size` >> rw []
+  WF_REL_TAC `measure $ texp_size (K 1)` >> rw []
 End
 
 Definition texp_wf_def[nocompute]:
@@ -70,7 +71,7 @@ Definition texp_wf_def[nocompute]:
     ¬ MEM gv (FLAT $ MAP (cepat_vars_l o FST) ((p,e) :: pes))) ∧
   texp_wf (UserAnnot _ e) = texp_wf e
 Termination
-  WF_REL_TAC `measure texp_size` >> rw[fetch "-" "texp_size_def"] >>
+  WF_REL_TAC `measure $ texp_size (K 1)` >> rw[fetch "-" "texp_size_def"] >>
   gvs[MEM_MAP, EXISTS_PROD] >>
   rename1 `MEM _ es` >> Induct_on `es` >> rw[] >> gvs[fetch "-" "texp_size_def"]
 End
@@ -78,16 +79,18 @@ End
 val texp_size_eq = fetch "-" "texp_size_eq";
 
 Theorem texp_size_lemma:
-  (∀xs v e. MEM (v,e) xs ⇒ texp_size e < texp1_size xs) ∧
-  (∀xs p e. MEM (p,e) xs ⇒ texp_size e < texp3_size xs) ∧
-  (∀xs a. MEM a xs ⇒ texp_size a < texp5_size xs)
+  (∀xs v e f. MEM (v,e) xs ⇒ texp_size f e < texp1_size f xs) ∧
+  (∀xs p e f. MEM (p,e) xs ⇒ texp_size f e < texp3_size f xs) ∧
+  (∀xs a f. MEM a xs ⇒ texp_size f a < texp5_size f xs)
 Proof
   rpt conj_tac
   \\ Induct \\ rw [] \\ fs [fetch "-" "texp_size_def"] \\ res_tac \\ fs []
+  \\ irule LESS_LESS_EQ_TRANS
+  \\ first_assum $ irule_at (Pos hd) \\ fs[]
 QED
 
 Theorem better_texp_induction =
-        TypeBase.induction_of “:texp”
+        TypeBase.induction_of “:'a texp”
           |> Q.SPECL [‘P’,
                       ‘λxs. ∀v e. MEM (v,e) xs ⇒ P e’,
                       ‘λ(v,e). P e’,
@@ -102,7 +105,7 @@ Theorem better_texp_induction =
 val _ = TypeBase.update_induction better_texp_induction
 
 Definition every_texp_def[simp]:
-  every_texp (p:texp -> bool) (Var cs v) = p (Var cs v) ∧
+  every_texp (p:'a texp -> bool) (Var cs v) = p (Var cs v) ∧
   every_texp p (Prim x es) =
     (p (Prim x es) ∧ EVERY (every_texp p) es) ∧
   every_texp p (App e es) =
@@ -120,7 +123,7 @@ Definition every_texp_def[simp]:
      EVERY (every_texp p) $ MAP SND rows) ∧
   every_texp p (UserAnnot t e) = (p (UserAnnot t e) ∧ every_texp p e)
 Termination
-  WF_REL_TAC ‘measure $ texp_size o SND’ >>
+  WF_REL_TAC ‘measure $ texp_size (K 1) o SND’ >>
   simp[texp_size_eq, MEM_MAP, PULL_EXISTS, FORALL_PROD] >> rw[] >>
   rename [‘MEM _ list’] >> Induct_on ‘list’ >>
   simp[FORALL_PROD, listTheory.list_size_def, basicSizeTheory.pair_size_def] >>
